Update examples syntax
Drop
- hclose
- tv/pv coercions
- unneeded non-HOAS variants of HOAS definitions

Remove now useless APIs and replace them. Replace:
- h?pN with h?xN.
- h?vabs' with h?vabs.
- λ:: with λ:

theories/Dot/examples/ex_utils.v
@@ -128,13 +128,6 @@ Notation x3 := (var_vl 3).
 Notation x4 := (var_vl 4).
 Notation x5 := (var_vl 5).
 
-Notation p0 := (pv x0).
-Notation p1 := (pv x1).
-Notation p2 := (pv x2).
-Notation p3 := (pv x3).
-Notation p4 := (pv x4).
-Notation p5 := (pv x5).
-
 Notation TUnit := (⊤%ty : ty).
 Notation tUnit := (tv (vint 0) : tm).
 
@@ -168,8 +161,7 @@ Hint Extern 0 (dms_hasnt _ _) => done : core.
 
 Hint Resolve Nat.lt_0_succ : core.
 
-Definition vabs' x := tv (vabs x).
-Definition lett t u := tapp (vabs' u) t.
+Definition lett t u := tapp (vabs u) t.
 
 (* Simplify substitution operations on concrete terms. *)
 Ltac simplSubst := rewrite /= /up/= /ids/ids_vl/=.
